code/rsapss/Hacl.RSAPSS.fst
@@ -1,5 +1,6 @@
 module Hacl.RSAPSS
 
+open FStar.Mul
 open Lib.IntTypes
 
 module S = Spec.RSAPSS
@@ -18,42 +19,68 @@ module BD = Hacl.Bignum.Definitions
 inline_for_extraction noextract
 let t_limbs = U64
 
+inline_for_extraction noextract
+let modBits_t = RI.modBits_t t_limbs
+
+inline_for_extraction noextract
+let ke (modBits:modBits_t) =
+  BE.mk_runtime_exp #t_limbs (BD.blocks modBits (size (bits t_limbs)))
+
+
 private
 [@CInline]
-let load_pkey : RK.rsapss_load_pkey_st t_limbs =
-  RK.rsapss_load_pkey RK.mk_runtime_rsapss_checks
+let load_pkey (modBits:modBits_t) : RK.rsapss_load_pkey_st t_limbs (ke modBits) modBits =
+  RK.rsapss_load_pkey (ke modBits) modBits RK.mk_runtime_rsapss_checks
 
 private
 [@CInline]
-let load_skey : RK.rsapss_load_skey_st t_limbs =
-  RK.rsapss_load_skey RK.mk_runtime_rsapss_checks load_pkey
+let load_skey (modBits:modBits_t) : RK.rsapss_load_skey_st t_limbs (ke modBits) modBits =
+  RK.rsapss_load_skey (ke modBits) modBits RK.mk_runtime_rsapss_checks (load_pkey modBits)
 
 
-val rsapss_sign: RI.rsapss_sign_st t_limbs
+val rsapss_sign:
+    a:Hash.algorithm{S.hash_is_supported a}
+  -> modBits:modBits_t ->
+  RI.rsapss_sign_st t_limbs (ke modBits) a modBits
+
 let rsapss_sign a modBits eBits dBits skey sLen salt msgLen msg sgnt =
-  RI.rsapss_sign a modBits eBits dBits skey sLen salt msgLen msg sgnt
+  RI.rsapss_sign (ke modBits) a modBits eBits dBits skey sLen salt msgLen msg sgnt
 
 
-val rsapss_verify: RI.rsapss_verify_st t_limbs
+val rsapss_verify:
+    a:Hash.algorithm{S.hash_is_supported a}
+  -> modBits:modBits_t ->
+  RI.rsapss_verify_st t_limbs (ke modBits) a modBits
+
 let rsapss_verify a modBits eBits pkey sLen k sgnt msgLen msg =
-  RI.rsapss_verify a modBits eBits pkey sLen k sgnt msgLen msg
+  RI.rsapss_verify (ke modBits) a modBits eBits pkey sLen k sgnt msgLen msg
 
 
-val new_rsapss_load_pkey: RK.new_rsapss_load_pkey_st t_limbs
-let new_rsapss_load_pkey r modBits eBits nb eb =
-  RK.new_rsapss_load_pkey load_pkey r modBits eBits nb eb
+val new_rsapss_load_pkey: modBits:modBits_t -> RK.new_rsapss_load_pkey_st t_limbs (ke modBits) modBits
+let new_rsapss_load_pkey modBits r eBits nb eb =
+  RK.new_rsapss_load_pkey (ke modBits) modBits (load_pkey modBits) r eBits nb eb
 
 
-val new_rsapss_load_skey: RK.new_rsapss_load_skey_st t_limbs
-let new_rsapss_load_skey r modBits eBits dBits nb eb db =
-  RK.new_rsapss_load_skey load_skey r modBits eBits dBits nb eb db
+val new_rsapss_load_skey: modBits:modBits_t -> RK.new_rsapss_load_skey_st t_limbs (ke modBits) modBits
+let new_rsapss_load_skey modBits r eBits dBits nb eb db =
+  RK.new_rsapss_load_skey (ke modBits) modBits (load_skey modBits) r eBits dBits nb eb db
 
 
-val rsapss_skey_sign: RI.rsapss_skey_sign_st t_limbs
+val rsapss_skey_sign:
+    a:Hash.algorithm{S.hash_is_supported a}
+  -> modBits:modBits_t ->
+  RI.rsapss_skey_sign_st t_limbs (ke modBits) a modBits
+
 let rsapss_skey_sign a modBits eBits dBits nb eb db sLen salt msgLen msg sgnt =
-  RI.rsapss_skey_sign load_skey rsapss_sign a modBits eBits dBits nb eb db sLen salt msgLen msg sgnt
+  RI.rsapss_skey_sign (ke modBits) a modBits
+    (load_skey modBits) (rsapss_sign a modBits) eBits dBits nb eb db sLen salt msgLen msg sgnt
 
 
-val rsapss_pkey_verify: RI.rsapss_pkey_verify_st t_limbs
+val rsapss_pkey_verify:
+    a:Hash.algorithm{S.hash_is_supported a}
+  -> modBits:modBits_t ->
+  RI.rsapss_pkey_verify_st t_limbs (ke modBits) a modBits
+
 let rsapss_pkey_verify a modBits eBits nb eb sLen k sgnt msgLen msg =
-  RI.rsapss_pkey_verify load_pkey rsapss_verify a modBits eBits nb eb sLen k sgnt msgLen msg
+  RI.rsapss_pkey_verify (ke modBits) a modBits
+    (load_pkey modBits) (rsapss_verify a modBits) eBits nb eb sLen k sgnt msgLen msg
